cp

low-level/Veritas.HashSet.fst
@@ -12,98 +12,43 @@ module U32 = FStar.UInt32
 module U64 = FStar.UInt64
 
 open FStar.HyperStack.ST
-
-let flush_interleaving = ()
-
-// ---
-
 open LowStar.BufferOps
-
-let hash_value_t = Hacl.Blake2b_32.lbytes 32
-let hash_value_buf = B.lbuffer u8 32
-
-// Relying on a somewhat recent kremlin optimization that removes pointers to unit
-noeq
-type state_s = {
-  acc: hash_value_buf;
-  seen: B.pointer (G.erased (list hashable_bytes));
-  key: key:B.buffer u8 { B.length key == 64 };
-  g_key: G.erased t_key;
-}
-
-let seen h s =
-  let s = B.deref h s in
-  G.reveal (B.deref h s.seen)
-
-let v h s =
-  let s = B.deref h s in
-  B.as_seq h s.acc
-
-let key s =
-  G.reveal s.g_key
-
-let footprint_s s =
-  B.(loc_addr_of_buffer s.acc `loc_union` loc_addr_of_buffer s.seen `loc_union` loc_addr_of_buffer s.key)
-
-unfold
-let invariant_s' h s =
-  B.live h s.acc /\ B.freeable s.acc /\
-  B.live h s.seen /\ B.freeable s.seen /\
-  B.live h s.key /\ B.freeable s.key /\
-  B.disjoint s.acc s.seen /\
-  B.disjoint s.acc s.key /\
-  B.disjoint s.seen s.key /\
-  B.as_seq h s.acc == gfold_right (fold_and_hash s.g_key) (G.reveal (B.deref h s.seen)) zero /\
-  G.reveal s.g_key == B.as_seq h s.key /\
-  B.as_seq h s.key `Seq.equal` Seq.create 64 0uy
-
-let invariant_s = invariant_s'
-
-let invariant_loc_in_footprint _ _ =
-  allow_inversion state_s
-
-let v_folds_seen _ _ =
-  ()
-
-let frame _ _ _ _ =
-  allow_inversion state_s
-
-#push-options "--ifuel 1 --fuel 1 --z3rlimit 50"
-let create_in r =
-  let b = B.malloc r 0uy 32ul in
-  let p = B.malloc r (G.hide ([] #hashable_bytes)) 1ul in
-  let k = B.malloc r 0uy 64ul in
-  let h0 = ST.get () in
-  [@inline_let]
-  let s: state_s = { acc = b; seen = p; key = k; g_key = B.as_seq h0 k } in
-  B.malloc r s 1ul
-#pop-options
-
 
 let hash_value (s:Seq.seq U8.t { Seq.length s <= blake2_max_input_length })
   : hash_value_t
-  = Hacl.Blake2b_32.spec s 64 (Seq.create 64 0uy) 32
+  = Hacl.Blake2b_32.spec s 0 Seq.empty 32
+
+noextract inline_for_extraction
+let xor_bytes (s1: Seq.seq U8.t)
+              (s2: Seq.seq U8.t { S.length s1 == S.length s2 })
+  : s3:Seq.seq U8.t { S.length s3 == S.length s1 }
+  = S.init (S.length s1) (fun i -> S.index s1 i `FStar.UInt8.logxor` S.index s2 i)
 
 let aggregate_hash_value (h0 h1: hash_value_t)
   : hash_value_t
   = xor_bytes h0 h1
 
-let as_hash_value (b:hash_value_buf) (h:HS.mem) =
-  B.as_seq h b
-
 let as_hash_value_pfx (b:hash_value_buf) (h:HS.mem) (n:nat { n <= 32 }) =
   Seq.slice (as_hash_value b h) 0 n
 
-val aggregate_hash_value_buf (b1: hash_value_buf) (b2: hash_value_buf)
-  : Stack unit
-    (requires fun h0 ->
-      B.live h0 b1 /\
-      B.live h0 b2 /\
-      B.disjoint b1 b2)
-    (ensures fun h0 _ h1 ->
-      B.(modifies (loc_buffer b1) h0 h1) /\
-      as_hash_value b1 h1 == aggregate_hash_value (as_hash_value b1 h0)
-                                                  (as_hash_value b2 h0))
+let state = hash_value_buf
+
+let invariant s h = B.live h s /\ B.freeable s
+
+let v_hash (s:state) (h:HS.mem)
+  : GTot hash_value_t
+  = as_hash_value s h
+
+let footprint s = B.loc_addr_of_buffer s
+
+let frame _ _ _ _ = ()
+
+////////////////////////////////////////////////////////////////////////////////
+
+(** Create an instance of a hash accumulator in the heap *)
+let create_in () = B.malloc HS.root 0uy 32ul
+
+////////////////////////////////////////////////////////////////////////////////
 let aggregate_hash_value_buf b1 b2 =
   let h0 = ST.get () in
   let inv h (i:nat) =
@@ -186,52 +131,33 @@ let aggregate_hash_value_buf b1 b2 =
   assert (as_hash_value b1 h ==
           aggregate_hash_value (as_hash_value b1 h0) (as_hash_value b2 h0))
 
-let v_hash (s:state) (h:HS.mem)
-  : GTot hash_value_t
-  = as_hash_value (B.get h s 0).acc h
-
-#push-options "--fuel 1 --z3rlimit 20 --query_stats"
+////////////////////////////////////////////////////////////////////////////////
 let add s b l =
-  let _ = allow_inversion state_s in
   let h0 = ST.get () in
   let b = B.sub b 0ul (Ghost.hide l) in
-  assert (invariant h0 s);
+  assert (invariant s h0);
   push_frame ();
-  let s0 = !* s in
-  let { acc; seen; key } = s0 in
+  let acc = s in
   let h1 = ST.get () in
-  assert (invariant h1 s);
+  assert (invariant s h1);
   let tmp = B.alloca 0uy 32ul in
   assert_norm (64 + Hacl.Blake2b_32.size_block < pow2 32);
   assert_norm (64 < pow2 32);
   assert_norm (64 <= Hacl.Blake2b_32.max_key);
-  Hacl.Blake2b_32.blake2b 32ul tmp l b 64ul key;
+  let h1' = ST.get () in
+  Hacl.Blake2b_32.blake2b 32ul tmp l b 0ul B.null;
   let h2 = ST.get () in
+  assert (B.as_seq h1' B.null `Seq.equal` Seq.empty #U8.t);
   assert (B.as_seq h2 tmp == hash_value (B.as_seq h1 b));
   aggregate_hash_value_buf acc tmp;
-  seen *= G.hide (B.as_seq h1 b :: B.deref h1 seen);
   let h = ST.get () in
   assert (v_hash s h ==
                 aggregate_hash_value (v_hash s h0)
                                      (hash_value (B.as_seq h0 b)));
   pop_frame ()
-#pop-options
 
-let get s =
-  let s = !*s in
-  let hash0 = B.sub s.acc 0ul 8ul in
-  let hash1 = B.sub s.acc 8ul 8ul in
-  let hash2 = B.sub s.acc 16ul 8ul in
-  let hash3 = B.sub s.acc 24ul 8ul in
-  let v0 = LowStar.Endianness.load64_le hash0 in
-  let v1 = LowStar.Endianness.load64_le hash1 in
-  let v2 = LowStar.Endianness.load64_le hash2 in
-  let v3 = LowStar.Endianness.load64_le hash3 in
-  { Veritas.Formats.Types.v0; Veritas.Formats.Types.v1; Veritas.Formats.Types.v2; Veritas.Formats.Types.v3 }
+////////////////////////////////////////////////////////////////////////////////
+let get s out = B.blit s 0ul out 0ul 32ul
 
-let free s =
-  let { seen; acc; key } = !* s in
-  B.free s;
-  B.free seen;
-  B.free acc;
-  B.free key
+////////////////////////////////////////////////////////////////////////////////
+let free s = B.free s
