low-level/Veritas.HashSet.fsti
@@ -13,15 +13,6 @@ module U64 = FStar.UInt64
 
 open FStar.HyperStack.ST
 
-inline_for_extraction noextract
-val flush_interleaving: unit
-
-noextract inline_for_extraction
-let u8 = FStar.UInt8.t
-
-noextract inline_for_extraction
-let bytes = S.seq u8
-
 // JP: not being agile over the hash algorithm for the moment, can be improved
 // later; any keyed hash will do, HMAC would also work, AES-CMAC is the one
 // currently used in Veritas
@@ -31,178 +22,97 @@ let bytes = S.seq u8
 // easily be 2 ^ 64 - 128.
 inline_for_extraction noextract
 let blake2_max_input_length = pow2 32 - 1 - 128
-inline_for_extraction noextract
-let blake2_key_length = 64
 
 // NOTE: we do not have an agile spec for the keyed hash functionality :(, so
 // we're making Blake2-dependent assumptions without corresponding agile predicates
 noextract inline_for_extraction
-let hashable_bytes = b:bytes { S.length b <= blake2_max_input_length }
+let hashable_bytes = s:Seq.seq U8.t { Seq.length s <= blake2_max_input_length }
+let hashable_buffer = b:B.buffer U8.t { B.length b <= blake2_max_input_length }
 
-noextract inline_for_extraction
-let lbytes = Hacl.Blake2b_32.lbytes
+let hash_value_t = Seq.lseq U8.t 32
 
-// NOTE: picking 32 bytes here, which gives a 256-bit hash. We could also do 64
-// bytes, the maximum allowed by Blake2.
-noextract inline_for_extraction
-let t = lbytes 32
-noextract inline_for_extraction
-let t_key = lbytes blake2_key_length
+val hash_value (_:hashable_bytes)
+  : hash_value_t
 
-// ---
+val aggregate_hash_value (_ _: hash_value_t)
+  : hash_value_t
+
+let hash_value_buf = B.lbuffer U8.t 32
+
+let as_hash_value (b:hash_value_buf) (h:HS.mem)
+  : GTot hash_value_t
+  = B.as_seq h b
 
 [@CAbstractStruct]
-val state_s: Type0
+val state: Type0
 
-let state = B.pointer state_s
+val invariant (s: state) (h:HS.mem) : Type0
 
-// ---
+val v_hash (s:state) (h:HS.mem)
+  : GTot hash_value_t
 
-val seen: h:HS.mem -> s:state -> GTot (list hashable_bytes)
-
-noextract inline_for_extraction
-let zero: t =
-  S.create 32 0uy
-
-val v: h:HS.mem -> s:state -> GTot t
-
-/// Combined with the modifies clause over only the footprint_s, clients should
-/// be able to deduce that the initial key is not modified.
-val key: s:state_s -> GTot t_key
-
-/// "As we all know", right folds are the easiest to work with because they
-/// follow the natural structure of recursion (left-folds are evil).
-///
-/// JP: is this defined somewhere?
-let rec gfold_right #a #b (f: b -> a -> GTot b) (xs: list a) (acc: b): Ghost b
-  (requires True)
-  (ensures fun _ -> True)
-  (decreases xs)
-=
-  let _ = allow_inversion (list a) in
-  match xs with
-  | [] -> acc
-  | x :: xs -> f (gfold_right f xs acc) x
-
-/// JP: is this defined somewhere?
-noextract inline_for_extraction
-let xor_bytes (s1: bytes) (s2: bytes { S.length s1 == S.length s2 }): s3:bytes { S.length s3 == S.length s1 } =
-  S.init (S.length s1) (fun i -> S.index s1 i `FStar.UInt8.logxor` S.index s2 i)
-
-let xor_bytes_commutative (s1: bytes) (s2: bytes { S.length s1 == S.length s2 }): Lemma
-  (ensures xor_bytes s1 s2 == xor_bytes s2 s1)
-  [ SMTPat (xor_bytes s1 s2) ]
-=
-  admit ()
-
-noextract inline_for_extraction
-let fold_and_hash (k: t_key) (acc: t) (b: hashable_bytes) =
-  xor_bytes (Hacl.Blake2b_32.spec b 64 k 32) acc
-
-// ---
-
-val footprint_s (s: state_s): GTot B.loc
-
-let footprint (h: HS.mem) (s: state) =
-  B.(loc_union (loc_addr_of_buffer s) (footprint_s (B.deref h s)))
-
-let loc_includes_union_l_footprint_s
-  (l1 l2: B.loc) (s: state_s)
-: Lemma
-  (requires (
-    B.loc_includes l1 (footprint_s s) \/ B.loc_includes l2 (footprint_s s)
-  ))
-  (ensures (B.loc_includes (B.loc_union l1 l2) (footprint_s s)))
-  [SMTPat (B.loc_includes (B.loc_union l1 l2) (footprint_s s))]
-= B.loc_includes_union_l l1 l2 (footprint_s s)
-
-val invariant_s (h: HS.mem) (s: state_s): Type0
-
-// JP: bolting in the fact that we only heap-allocate this state
-let invariant (h: HS.mem) (s: state) =
-  invariant_s h (B.deref h s) /\
-  B.live h s /\
-  B.freeable s /\
-  B.(loc_disjoint (loc_addr_of_buffer s) (footprint_s (B.deref h s)))
-
-val invariant_loc_in_footprint
-  (h: HS.mem)
-  (s: state)
-: Lemma
-  (requires (invariant h s))
-  (ensures (B.loc_in (footprint h s) h))
-  [SMTPat (invariant h s)]
-
-// ---
-
-val v_folds_seen (h: HS.mem) (s: state): Lemma
-  (requires (
-    invariant h s))
-  (ensures (
-    v h s == gfold_right (fold_and_hash (key (B.deref h s))) (seen h s) zero))
-  [ SMTPat (invariant h s) ]
+(** A bunch of infrastructure related to framing **)
+val footprint (s: state): GTot B.loc
 
 val frame: l:B.loc -> s:state -> h0:HS.mem -> h1:HS.mem -> Lemma
   (requires (
-    invariant h0 s /\
-    B.loc_disjoint l (footprint h0 s) /\
+    invariant s h0 /\
+    B.loc_disjoint l (footprint s) /\
     B.modifies l h0 h1))
   (ensures (
-    invariant h1 s /\
-    footprint h0 s == footprint h1 s /\
-    v h0 s == v h1 s /\
-    seen h0 s == seen h1 s))
-  [ SMTPat (invariant h1 s); SMTPat (B.modifies l h0 h1) ]
+    invariant s h1 /\
+    v_hash s h0 == v_hash s h1))
 
-// ---
+(*** THE MAIN INTERFACE ***)
 
-val create_in: r:HS.rid -> ST state
-  (requires (fun h0 ->
-    HyperStack.ST.is_eternal_region r))
-  (ensures (fun h0 s h1 ->
-    invariant h1 s /\
-    seen h1 s == [] /\
+(** Create an instance of a hash accumulator in the heap *)
+val create_in: unit -> ST state
+  (requires fun h0 -> True)
+  (ensures fun h0 s h1 ->
+    invariant s h1 /\
     B.(modifies loc_none h0 h1) /\
-    B.fresh_loc (footprint h1 s) h0 h1 /\
-    B.(loc_includes (loc_region_only true r) (footprint h1 s))))
+    B.fresh_loc (footprint s) h0 h1)
 
-val add: s:state -> b:B.buffer u8 -> l:U32.t -> Stack unit
-  (requires (fun h0 ->
-    invariant h0 s /\
-    U32.v (B.len b) >= U32.v l /\
-    B.live h0 b /\
-    U32.v l <= blake2_max_input_length /\
-    // Note: this is blake2 specific.
-    B.(loc_disjoint (loc_buffer b) (footprint h0 s))))
-  (ensures (fun h0 _ h1 ->
-    invariant h1 s /\
-    B.modifies (footprint_s (B.deref h0 s)) h0 h1 /\
-    // FYI, no need to talk about a preserved footprint since I used footprint_s
-    // which is not heap-dependent
-    seen h1 s == B.as_seq h0 (B.gsub b 0ul l) :: seen h0 s))
+(** Combine two hash values held in b1 and b2 into b1 *)
+val aggregate_hash_value_buf (b1: hash_value_buf) (b2: hash_value_buf)
+  : Stack unit
+    (requires fun h0 ->
+      B.live h0 b1 /\
+      B.live h0 b2 /\
+      B.disjoint b1 b2)
+    (ensures fun h0 _ h1 ->
+      B.(modifies (loc_buffer b1) h0 h1) /\
+      as_hash_value b1 h1 == aggregate_hash_value (as_hash_value b1 h0)
+                                                  (as_hash_value b2 h0))
 
-inline_for_extraction noextract
-let u256 = Veritas.Formats.Types.u256
+(** Hash the (input[0, l)) into the hash accumulate s *)
+val add: s:state -> input:hashable_buffer -> l:U32.t -> Stack unit
+  (requires fun h0 ->
+    invariant s h0 /\
+    B.live h0 input /\
+    B.(loc_disjoint (loc_buffer input) (footprint s)) /\
+    U32.v l <= U32.v (B.len input))
+  (ensures fun h0 _ h1 ->
+    invariant s h1 /\
+    B.modifies (footprint s) h0 h1 /\
+    v_hash s h1 ==
+    aggregate_hash_value (v_hash s h0)
+                         (hash_value (Seq.slice (B.as_seq h0 input) 0 (U32.v l))))
 
-inline_for_extraction noextract
-let u256_of_blake2_hash (hash: lbytes 32): u256 =
-  let hash12, hash34 = S.split hash 16 in
-  let hash1, hash2 = S.split hash12 8 in
-  let hash3, hash4 = S.split hash34 8 in {
-    Veritas.Formats.Types.v0 = FStar.Endianness.uint64_of_le hash1;
-    Veritas.Formats.Types.v1 = FStar.Endianness.uint64_of_le hash2;
-    Veritas.Formats.Types.v2 = FStar.Endianness.uint64_of_le hash3;
-    Veritas.Formats.Types.v3 = FStar.Endianness.uint64_of_le hash4
-  }
-
-val get: s:state -> Stack u256
-  (requires fun h0 -> invariant h0 s)
+(** Read the current value of the hash into out *)
+val get: s:state -> out:hash_value_buf -> Stack unit
+  (requires fun h0 ->
+    invariant s h0 /\
+    B.live h0 out /\
+    B.loc_disjoint (B.loc_buffer out) (footprint s))
   (ensures fun h0 r h1 ->
-    h0 == h1 /\
-    r == u256_of_blake2_hash (v h0 s))
+    invariant s h0 /\
+    B.modifies (B.loc_buffer out) h0 h1 /\
+    v_hash s h0 == as_hash_value out h1)
 
+(** Free the hash accumulator *)
 val free: s:state -> ST unit
-  (requires (fun h0 ->
-    invariant h0 s))
+  (requires fun h0 ->
+    invariant s h0)
   (ensures (fun h0 _ h1 ->
-    B.modifies (footprint h0 s) h0 h1))
+    B.modifies (footprint s) h0 h1))
